

5. Prove the estimate (12.23).

[Hint: for each internal node x_j , $j = 1, \dots, n-1$, integrate by parts (12.21) to get

$$\tau_h(x_j)$$

$$= -u''(x_j) - \frac{1}{h^2} \left[\int_{x_j-h}^{x_j} u''(t)(x_j-h-t)^2 dt - \int_{x_j}^{x_j+h} u''(t)(x_j+h-t)^2 dt \right].$$

Then, pass to the squares and sum $\tau_h(x_j)^2$ for $j = 1, \dots, n-1$. On noting that $(a+b+c)^2 \leq 3(a^2+b^2+c^2)$, for any real numbers a, b, c , and applying the Cauchy-Schwarz inequality yields the desired result.]

from 12.21

$$\tau_h(x_j) = \frac{1}{h^2} \left(\int_{x_j-h}^{x_j+h} (u'''(t) - u'''(x_j)) \frac{(x_j+h-t)^2}{2} dt - \int_{x_j-h}^{x_j} (u'''(t) - u'''(x_j)) \frac{(x_j-h-t)^2}{2} dt \right)$$

$$\stackrel{\text{IBP}}{=} -u''(x_j) - \frac{1}{h^2} \left(\int_{x_j-h}^{x_j} u'''(t)(x_j-h-t)^2 dt - \int_{x_j}^{x_j+h} u'''(t)(x_j+h-t)^2 dt \right)$$

$$\stackrel{\text{let}}{=} a_j + b_j + c_j, \quad a_j = -u''(x_j), \quad b_j = \frac{1}{h^2} \int_{x_j-h}^{x_j} u'''(t)(x_j-h-t)^2 dt$$

$$c_j = \frac{1}{h^2} \int_{x_j}^{x_j+h} u'''(t)(x_j+h-t)^2 dt$$

$$b_j^2 \leq \int_{x_j-h}^{x_j} (u'''(t))^2 dt \cdot \int_{x_j-h}^{x_j} (x_j-h-t)^4 dt = \frac{h}{5} \int_{x_j-h}^{x_j} (u'''(t))^2 dt$$

$$c_j^2 \leq \frac{h}{5} \int_{x_j}^{x_j+h} (u'''(t))^2 dt$$

$$\Rightarrow \|\tau_h\|_h^2 = h \sum_{j=1}^{n-1} |\tau_h(x_j)|^2 = h \sum_{j=1}^{n-1} (a_j + b_j + c_j)^2$$

$$\leq h \sum_{j=1}^{n-1} 3(a_j + b_j + c_j) = 3 \left(h \sum_{j=1}^{n-1} a_j + \frac{2h}{5} \|u'''\|_{L(\omega_1)}^2 \right)$$

$$\leq 3 \left(\|u'\|_h^2 + \|u''\|_{L(\omega_1)}^2 \right) \stackrel{-u''=f}{=} 3 \left(\|u'\|_h^2 + \|f\|_{L(\omega_1)}^2 \right)$$

7. Let $g = 1$ and prove that $T_h g(x_j) = \frac{1}{2} x_j (1 - x_j)$.
 [Solution: use the definition (12.25) with $g(x_k) = 1$, $k = 1, \dots, n-1$ and recall that $G^k(x_j) = hG(x_j, x_k)$ from the exercise above. Then

$$T_h g(x_j) = h \left[\sum_{k=1}^j x_k (1 - x_j) + \sum_{k=j+1}^{n-1} x_j (1 - x_k) \right]$$

from which, after straightforward computations, one gets the desired result.]

$$g(x_k) = 1$$

$$\begin{aligned} T_h g(x_j) &= \sum_{k=1}^{n-1} g(x_k) G^k = \sum_{k=1}^{n-1} h g(x_k) G(x_j, x_k) = h \sum_{k=1}^{n-1} G(x_j, x_k) \\ &= h \left(\sum_{k=1}^j G(x_j, x_k) + \sum_{k=j+1}^{n-1} G(x_j, x_k) \right) \\ &= h \left(\sum_{k=1}^j x_k (1 - x_j) + \sum_{k=j+1}^{n-1} x_j (1 - x_k) \right), \quad G(x_j, x_k) = \begin{cases} x_k (1 - x_j), & x_k \leq x_j \\ x_j (1 - x_k), & x_k > x_j \end{cases} \\ &= h \left(\sum_{k=1}^j k h (1 - h_j) + \sum_{k=j+1}^{n-1} h_j (1 - k h) \right) \\ &= h \left(j \left(\frac{1+j}{2} \right) h (1 - h_j) + h_j \left((n-j-1) - h \left(\frac{n+j}{2} \right) (n-j-1) \right) \right) \\ &= h^2 j \left(\frac{1}{2} (1+j) (1 - h_j) + n-j-1 - \frac{1}{2} (n+j) (n-j-1) \right) \\ &= \frac{h^2 j}{2} (1+j - h_j - h_j^2 + 2n-2j-2 - n^2 h - n h + j^2 h + j h) \quad , \quad n = \frac{1}{h} \\ &= \frac{h^2 j}{2} \left(j + \frac{1}{h} \right) = \frac{h j}{2} (1 + h_j) = \frac{1}{2} x_j (1 + x_j) \end{aligned}$$

8. Prove Young's inequality (12.40).

$$\because \left(\sqrt{\varepsilon}a - \frac{1}{\sqrt{\varepsilon}}b\right)^2 \geq 0, \quad a, b \in \mathbb{R}, \quad \varepsilon > 0$$

$$\Rightarrow \varepsilon a^2 - ab + \frac{b^2}{4\varepsilon} \geq 0$$

$$\Rightarrow ab \leq \varepsilon a^2 + \frac{b^2}{4\varepsilon}$$

9. Show that $\|v_h\|_h \leq \|v_h\|_{h,\infty} \quad \forall v_h \in V_h$.

$$\begin{aligned} \because \|v_h\|_h^2 &= h \sum_{k=1}^{n-1} V_h^2(x_k) \leq h \sum_{k=1}^{n-1} \max_{1 \leq k \leq n-1} V_h^2(x_k) = h \sum_{k=1}^{n-1} \|v_h\|_{h,\infty}^2 \\ &= \frac{1}{n} (n-1) \|v_h\|_{h,\infty}^2 \leq \|v_h\|_{h,\infty}^2 \end{aligned}$$

$$\therefore \|v_h\|_h \leq \|v_h\|_{h,\infty}, \quad \forall v_h \in V_h$$

11. Discretize the fourth-order differential operator $Lu(x) = -u^{(iv)}(x)$ using centered finite differences.

[*Solution*: apply twice the second order centered finite difference operator L_h defined in (12.9).]

$$L_h u_j = -\frac{1}{h^2} (u_{j+1} - 2u_j + u_{j-1})$$

$$\Rightarrow L_h(L_h u_h) = -\frac{1}{h^2} (L_h u_{j+1} - 2L_h u_j + L_h u_{j-1})$$

$$= \frac{1}{h^4} (u_{j+2} - 2u_{j+1} + u_j + u_j - 2u_{j-1} + u_{j-2} - 2u_{j+1} + 4u_j - 2u_{j-1})$$

$$= \frac{1}{h^4} (u_{j+2} - 4u_{j+1} + 6u_j - 4u_{j-1} + u_{j-2})$$